progress in FirstOrder

theories/Firstorder.v
@@ -1,7 +1,7 @@
 Require Import ssreflect Eqdep_dec.
 From MetaCoq.Utils Require Import All_Forall MCSquash MCList.
-From MetaCoq.Common Require Import config Kernames.
-From MetaCoq.PCUIC Require Import PCUICAst PCUICTyping PCUICFirstorder.
+From MetaCoq.Common Require Import Transform config Kernames.
+From MetaCoq.PCUIC Require Import PCUICAst PCUICTyping PCUICFirstorder PCUICCasesHelper.
 From MetaCoq.Erasure Require Import EWcbvEval EWcbvEvalNamed.
 From MetaCoq.SafeChecker Require Import PCUICErrors PCUICWfEnv PCUICWfEnvImpl.
 
@@ -9,7 +9,9 @@ From Malfunction Require Import Malfunction SemanticsSpec utils_array Compile.
 
 Require Import ZArith Array.PArray List String Floats Lia Bool.
 Import ListNotations.
+From MetaCoq.Utils Require Import bytestring.
 
+Print nat_rect.
 
 Unset Elimination Schemes. 
 
@@ -76,28 +78,45 @@ Section Realizability.
   
   Definition global_adt_decl := list (kername * realize_adt_type).
 
+  Open Scope bs. 
+
+  Definition empty_locals : Ident.Map.t := fun _ => fail "not_defined".
+
+  Close Scope bs. 
+
   Section Values. 
 
     Variable local_adt : list (value -> Prop).
     Variable global_adt : global_adt_decl.
-  
-    Definition realize_val (A:camlType) : value -> Prop.
+
+    Definition to_realize_term (realize_val : value -> Prop) 
+      : t -> Prop := fun t => forall h h' v, 
+      eval _ globals empty_locals h t h' v -> realize_val v.
+
+    Definition to_realize_value (realize_term : t -> Prop) 
+      : value -> Prop := fun v => exists t h h', 
+        eval _ globals empty_locals h t h' v /\ realize_term t.
+
+    Definition realize_term (A:camlType) : t -> Prop.
     Proof.
       refine (camlType_rect _ _ _ _ A); clear A.
       - intros A PA B PB.
-        refine (fun f => 
-              exists locals' x t, f = Func (locals',x,t) /\ 
-                forall v v' h h', 
-                    PA v -> 
-                    eval _ globals (Ident.Map.add x v locals') h t h' v' ->
-                    PB v').
-      - intros n. refine (List.nth n local_adt (fun _ => False)).
+        exact (fun f => forall t, PA t -> PB (Mapply(f,[t]))).
+      - intros n. 
+        exact (to_realize_term (List.nth n local_adt (fun _ => False))).
       - intros kn n params PAll.
         case (find (fun '(kn',_) => eq_kername kn kn') global_adt).
-        + intros [_ Hrel]. exact (Hrel params PAll (int_to_nat n)).
+        + intros [_ Hrel]. 
+          refine (to_realize_term (Hrel params _ (int_to_nat n))).
+          induction PAll; econstructor; eauto. eapply to_realize_value; eassumption.
         + intros; exact False. 
     Defined.
+
+    Definition realize_value (A:camlType) : value -> Prop :=
+      to_realize_value (realize_term A).
+
   End Values. 
+  MetaCoq Quote Recursively Definition tnat := nat.
 
   Fixpoint realize_ADT_gen_fix (global_adt : global_adt_decl) 
     (adt : list (list (list camlType))) (step : nat) : realize_adt_type.
@@ -116,7 +135,7 @@ Section Realizability.
           | _ => true end) constr_list).
       refine (Existsi (fun index Ts => 
           exists vs, v = Block (int_of_nat index, vs) /\ _) 0 constr_arg). 
-      refine (Forall2 (realize_val _ global_adt) Ts vs).
+      refine (Forall2 (realize_value _ global_adt) Ts vs).
       refine (_ ++ _).
       + (* parameters *)
         clear -paramRel. induction paramRel; [exact []| ].
@@ -150,7 +169,7 @@ Section firstorder.
     unfold firstorder_type. destruct (fst _).
     all: try solve [inversion 1].
     (* case of tRel with a valid index *)
-    - intro; exact (Rel n0).
+    - intro; exact (Rel (n0-n)).
     (* case of tInd where Σb is saying that inductive_mind is first order *)
     - intro; destruct ind. exact (Adt inductive_mind (int_of_nat inductive_ind) []).
   Defined.  
@@ -442,7 +461,7 @@ ind_universes0 ind_variance0) x Hparam Hfo'); eauto.
     ind_params mind = [] -> 
     is_true (forallb (@firstorder_oneind Σb mind) (ind_bodies mind)) -> ADT :=
     fun Hparam H => (0, CoqType_to_camlType' mind Hparam H).
-  
+
   Definition empty_heap : CanonicalHeap.(heapGen) (@SemanticsSpec.value CanonicalHeap) :=
     (int_of_nat 0 , fun _ => []).
 
@@ -457,59 +476,44 @@ ind_universes0 ind_variance0) x Hparam Hfo'); eauto.
         destruct (nth_error (EAst.ind_bodies m) ind); now inversion H.  
       + apply IHΣ; eauto.
   Qed.
+                  
+  Fixpoint zip {A B} (l:list A) (l':list B) : list (A * B) :=
+  match l , l' with 
+  | [] , [] => []
+  | a::l , b::l' => ((a,b) :: zip l l')
+  | _ , _ => [] 
+  end. 
+    
+  Lemma zip_length {A B} (l:list A) (l':list B) : 
+    #|l| = #|l'| ->  #|zip l l'| = #|l|.
+  Proof. 
+    revert l'; induction l; destruct l'; cbn; eauto.
+    intro Heq; inversion Heq. rewrite IHl; eauto.  
+  Qed. 
 
+  Lemma zip_fst {A B} (l:list A) (l':list B) : 
+    #|l| = #|l'| -> map fst (zip l l') = l.
+  revert l'; induction l; destruct l'; cbn; eauto.
+  - inversion 1.
+  - intro Heq; inversion Heq. rewrite IHl; eauto.
+  Qed.         
 
-  Lemma filter_length_nil ind k mind Eind Hparam Hfo :
-    let Emind := ErasureFunction.erase_mutual_inductive_body mind in 
-    nth_error (EAst.ind_bodies Emind) ind = Some Eind ->
-  List.length
-  (filter (fun x0 : nat =>  match x0 with
-      | 0 => true
-      | S _ => false
-      end)
-     (firstn k (map EAst.cstr_nargs (EAst.ind_ctors Eind)))) = 
-  List.length
-           (filter (fun x : list camlType =>
-               match x with
-               | [] => true
-               | _ :: _ => false
-               end)
-              (firstn k
-                 (nth ind
-                    (CoqType_to_camlType' mind
-                       Hparam Hfo) []))).
-    Admitted.                       
+  Lemma zip_snd {A B} (l:list A) (l':list B) : 
+  #|l| = #|l'| -> map snd (zip l l') = l'.
+  revert l'; induction l; destruct l'; cbn; eauto.
+  - inversion 1.  
+  - intro Heq; inversion Heq. rewrite IHl; eauto.
+  Qed.  
 
-    Lemma filter_length_not_nil ind k mind Eind Hparam Hfo :
-    let Emind := ErasureFunction.erase_mutual_inductive_body mind in 
-    nth_error (EAst.ind_bodies Emind) ind = Some Eind ->
-  List.length
-  (filter (fun x0 : nat =>  match x0 with
-      | 0 => false
-      | S _ => true 
-      end)
-     (firstn k (map EAst.cstr_nargs (EAst.ind_ctors Eind)))) = 
-  List.length
-           (filter (fun x : list camlType =>
-               match x with
-               | [] => false
-               | _ :: _ => true
-               end)
-              (firstn k
-                 (nth ind
-                    (CoqType_to_camlType' mind
-                       Hparam Hfo) []))).
-    Admitted.                       
-
-  Fixpoint All_exists T A P l 
-    (H: Forall (fun t : T => exists a : A, P t a) l) 
-    : exists l' : list A, Forall2 P l l'.
+  Fixpoint All_exists T U A P l l'
+    (H: Forall2 (fun (t : T) (u : U) => exists a : A, P t u a) l l')  
+    : exists l'' : list A, Forall2 (fun tu a => P (fst tu) (snd tu) a) (zip l l') l''.
   Proof. 
     destruct H.
     - exists []. econstructor.
-    - refine (let '(ex_intro l' X) := 
-              All_exists T A P _ H0 in _).
-      destruct H as [p H].
+    - destruct H as [p H].
+      refine (let '(ex_intro l' X) := 
+              All_exists T U A P _ _ H0 in _).
       exists (p::l'). econstructor; eauto. 
   Qed. 
 
@@ -559,12 +563,36 @@ ind_universes0 ind_variance0) x Hparam Hfo'); eauto.
   cbn. now f_equal.
   Qed. 
 
+  Lemma CoqType_to_camlType_oneind_nth mind Hparam x Hfo k l :
+  nth_error (CoqType_to_camlType_oneind mind x Hparam Hfo) k = Some l
+  -> exists l', nth_error (ind_ctors x) k = Some l' /\ #|l| = #|cstr_args l'|.
+  Proof.
+    destruct x; cbn. destruct MCProd.andb_and.
+    destruct (a Hfo). clear.
+    revert k l. induction ind_ctors0; cbn; eauto.
+    - intros k l H. rewrite nth_error_nil in H. inversion H.
+    - destruct MCProd.andb_and. destruct (a0 i0).
+      destruct a. intros k l H. destruct k; cbn. 
+      + eexists; split; [reflexivity |]. cbn in *.
+        inversion H. rewrite CoqType_to_camlType_ind_ctors_length.
+        rewrite Hparam. rewrite app_nil_r. apply rev_length.
+      + cbn in *. now eapply IHind_ctors0. 
+  Qed. 
+
   Lemma Forall_Forall2_and_inv {A B : Type} 
     {R : A -> B -> Prop} {P : A -> Prop} l l':
   Forall2 (fun (x : A) (y : B) => P x /\ R x y ) l l' ->
   Forall2 R l l' /\ Forall P l.
   Proof. 
     induction 1; repeat econstructor; now eauto.
+  Qed.
+
+  Lemma Forall2_forall {A B X: Type} 
+    {R : A -> B -> X -> Prop} l l':
+  Forall2 (fun a b => forall x, R a b x) l l' ->
+  forall x, Forall2 (fun a b => R a b x) l l'.
+  Proof.
+    induction 1; econstructor; eauto.
   Qed.
 
   Axiom cstr_arity_length : forall x, cstr_arity x = List.length (cstr_args x).
@@ -575,23 +603,255 @@ ind_universes0 ind_variance0) x Hparam Hfo'); eauto.
   Axiom ind_ctors_wB : forall mind j ind,
     nth_error mind j = Some ind ->
     #|ind_ctors ind| <= Z.to_nat Uint63.wB.
+  Axiom ind_wB : forall mind retro kn univ (cf:=config.extraction_checker_flags),
+    let Σ := mk_global_env univ [(kn , InductiveDecl mind)] retro in
+    PCUICTyping.wf Σ ->
+    #|ind_bodies mind| <= Z.to_nat Uint63.wB.
 
-  Definition camlValue_to_CoqValue_nil `{WcbvFlags} kn mind Eind 
-    (Hparam : ind_params mind = [])
-    (Hnparam : ind_npars mind = 0)
-    (Hfo : is_true (forallb (@firstorder_oneind Σb mind) (ind_bodies mind))) ind v :
-    let adt := CoqType_to_camlType mind Hparam Hfo in
-    let Emind := ErasureFunction.erase_mutual_inductive_body mind in 
-    let Σ := [(kn , EAst.InductiveDecl Emind)] in
-    with_constructor_as_block = true ->
-    ind < List.length (snd adt) ->
-    EGlobalEnv.lookup_inductive Σ (mkInd kn ind) = Some (Emind, Eind) ->
-    realize_ADT CanonicalHeap [] [] adt [] All_nil ind v ->
-    exists t, ∥ EWcbvEval.value Σ t ∥ /\ 
-    eval CanonicalHeap [] (fun _ => not_evaluated) empty_heap (compile Σ t) empty_heap v.
+  Axiom compile_pipeline : global_declarations -> term -> t.
+
+  Definition cstr_nargs : constructor_body -> nat := fun c => #| cstr_args c|.
+
+  Definition lookup_constructor_args Σ ind : option (list nat) 
+    := match lookup_inductive Σ ind with
+    | Some (_, idecl) => Some (map cstr_nargs (ind_ctors idecl))
+   | None => None
+    end.
+
+  Axiom compile_pipeline_tConstruct_nil : forall Σ i n inst, 
+    compile_pipeline Σ.(declarations) (tConstruct i n inst) = 
+    match lookup_constructor_args Σ i with
+    | Some num_args =>
+      Mnum (numconst_Int (int_of_nat (nonblocks_until n num_args)))
+    | None => Mstring "error: inductive not found"
+    end.
+
+  Axiom compile_pipeline_tConstruct_cons : forall Σ i n inst l, 
+    #|l| > 0 ->
+    compile_pipeline Σ.(declarations) (mkApps (tConstruct i n inst) l) =
+    match lookup_constructor_args Σ i with
+    | Some num_args =>
+      Mblock
+        (int_of_nat (blocks_until n num_args),
+         map_InP l (fun (x : term) (_ : In x l) => compile_pipeline Σ.(declarations) x))
+    | None => Mstring "error: inductive not found"
+    end.
+
+
+  Lemma filter_length_nil ind k mind Eind Hparam Hfo :
+    nth_error (ind_bodies mind) ind = Some Eind ->
+  List.length
+  (filter (fun x0 : nat =>  match x0 with
+      | 0 => true
+      | S _ => false
+      end)
+     (firstn k (map cstr_nargs (ind_ctors Eind)))) = 
+  List.length
+           (filter (fun x : list camlType =>
+               match x with
+               | [] => true
+               | _ :: _ => false
+               end)
+              (firstn k
+                 (nth ind
+                    (CoqType_to_camlType' mind
+                       Hparam Hfo) []))).
+    Admitted.                       
+
+    Lemma filter_length_not_nil ind k mind Eind Hparam Hfo :
+    nth_error (ind_bodies mind) ind = Some Eind ->
+  List.length
+  (filter (fun x0 : nat =>  match x0 with
+      | 0 => false
+      | S _ => true 
+      end)
+     (firstn k (map cstr_nargs (ind_ctors Eind)))) = 
+  List.length
+           (filter (fun x : list camlType =>
+               match x with
+               | [] => false
+               | _ :: _ => true
+               end)
+              (firstn k
+                 (nth ind
+                    (CoqType_to_camlType' mind
+                       Hparam Hfo) []))).
+    Admitted.     
+
+  Lemma Forall2_map_left {A B C} (P : A -> B -> Prop) (f : C -> A) (l : list C) (l' : list B) :
+    Forall2 P (map f l) l' <-> Forall2 (fun x y => P (f x) y) l l'.
+Proof.
+  split; intros.
+  + eapply Forall2_map_inv. now rewrite map_id.
+  + rewrite -(map_id l'). now eapply Forall2_map.
+Qed.
+
+End firstorder.
+
+Lemma CoqType_to_camlType_oneind_type_Rel n k decl_type Hfo :
+let T := CoqType_to_camlType_oneind_type (Σb := []) k n decl_type Hfo in
+exists i,  (k <= i) /\ (i < n + k) /\ T = Rel (i-k).
+Proof.
+unfold CoqType_to_camlType_oneind_type.
+unfold firstorder_type in Hfo.
+set (fst (PCUICAstUtils.decompose_app decl_type)) in *.
+destruct t; inversion Hfo; cbn; eauto.
+- apply MCProd.andb_and in H0. destruct H0. apply leb_complete in H, H0.
+  exists n0; repeat split; eauto.
+- destruct ind. inversion Hfo.
+Qed.   
+
+Lemma CoqType_to_camlType_oneind_Rel mind ind Hparam Hfo larg T k : 
+In larg (CoqType_to_camlType_oneind (Σb := []) mind ind Hparam Hfo) ->
+nth_error larg k = Some T -> exists i, (k <= i) /\ (i < #| ind_bodies mind| + k) /\ T = Rel (i-k).
+Proof. 
+destruct mind, ind. revert k Hfo. induction ind_ctors0; intros k Hfo Hlarg HT.
+- cbn in *; destruct MCProd.andb_and. destruct (a Hfo). destruct (in_nil Hlarg).
+- cbn; cbn in Hlarg. destruct MCProd.andb_and. cbn in Hfo. destruct (a0 Hfo). 
+  destruct MCProd.andb_and. destruct (a1 i0). destruct a.
+  unfold In in Hlarg. destruct Hlarg.
+  2: { eapply IHind_ctors0; eauto. cbn. destruct MCProd.andb_and.
+        destruct (a _). rewrite (bool_irr _ i6 i4). eauto.
+        Unshelve.
+        cbn. apply MCProd.andb_and. split; cbn; eauto. }
+  cbn in Hparam, i3. rewrite Hparam in i3, H. rewrite app_nil_r in i3, H.
+  clear - i3 HT H. set (rev cstr_args0) in *. rewrite <- H in HT. 
+  revert T HT. clear H.
+  cbn; set (Datatypes.length ind_bodies0) in *. 
+  setoid_rewrite <- (Nat.sub_0_r k) at 1. assert (k >= 0) by lia. revert H.  
+  revert k i3. generalize 0 at 1 2 3 4.
+  induction l; cbn; intros. 1: { apply nth_error_In in HT; inversion HT. }
+  destruct MCProd.andb_and. destruct (a0 i3). destruct a. 
+  unfold In in HT.
+  case_eq (k-n0); cbn in HT. 
+  + intro Heq. rewrite Heq in HT. inversion HT. unshelve epose (CoqType_to_camlType_oneind_type_Rel _ _ _ _).
+    5: erewrite H1 in e. rewrite H1. destruct e as [i2 [? [? ?]]]. exists (i2-(k - n0)).
+    repeat split. all: try lia. rewrite H3; f_equal. lia.  
+  + intros ? Heq. eapply IHl.
+    2: { rewrite Heq in HT. cbn in HT.  
+         assert (k - S n0 = n1) by lia. now erewrite H0. }
+    lia. 
+Qed. 
+
+Lemma CoqType_to_camlType'_unfold mind Hparam Hfo l : 
+In l (CoqType_to_camlType' (Σb := []) mind Hparam Hfo) ->
+exists ind Hfo', l =  CoqType_to_camlType_oneind (Σb := []) mind ind Hparam Hfo'.
+Proof.
+  destruct mind; cbn in *. revert Hfo.
+  enough (forall ind_bodies1, forall
+  Hfo : is_true
+          (forallb
+             (firstorder_oneind
+                {|
+                  Erasure.P.PCUICEnvironment.ind_finite := ind_finite0;
+                  Erasure.P.PCUICEnvironment.ind_npars := ind_npars0;
+                  Erasure.P.PCUICEnvironment.ind_params := ind_params0;
+                  Erasure.P.PCUICEnvironment.ind_bodies := ind_bodies1;
+                  Erasure.P.PCUICEnvironment.ind_universes := ind_universes0;
+                  Erasure.P.PCUICEnvironment.ind_variance := ind_variance0
+                |}) ind_bodies0),
+In l
+  (CoqType_to_camlType_fix (Σb := []) ind_bodies0 ind_finite0 ind_params0 ind_npars0 ind_universes0 ind_variance0
+     Hparam ind_bodies1 Hfo) ->
+exists
+  (ind : one_inductive_body) (Hfo' : is_true
+                                       (firstorder_oneind
+                                          {|
+                                            Erasure.P.PCUICEnvironment.ind_finite := ind_finite0;
+                                            Erasure.P.PCUICEnvironment.ind_npars := ind_npars0;
+                                            Erasure.P.PCUICEnvironment.ind_params := ind_params0;
+                                            Erasure.P.PCUICEnvironment.ind_bodies := ind_bodies1;
+                                            Erasure.P.PCUICEnvironment.ind_universes := ind_universes0;
+                                            Erasure.P.PCUICEnvironment.ind_variance := ind_variance0
+                                          |} ind)),
+  l =
+  CoqType_to_camlType_oneind (Σb := [])
+    {|
+      Erasure.P.PCUICEnvironment.ind_finite := ind_finite0;
+      Erasure.P.PCUICEnvironment.ind_npars := ind_npars0;
+      Erasure.P.PCUICEnvironment.ind_params := ind_params0;
+      Erasure.P.PCUICEnvironment.ind_bodies := ind_bodies1;
+      Erasure.P.PCUICEnvironment.ind_universes := ind_universes0;
+      Erasure.P.PCUICEnvironment.ind_variance := ind_variance0
+    |} ind Hparam Hfo').
+  { eapply H; eauto. }
+  induction ind_bodies0; cbn; intros.
+  - inversion H.
+  - destruct MCProd.andb_and. destruct (a0 Hfo). destruct H.
+    + exists a. now exists i0.
+    + eapply IHind_bodies0; eauto.
+  Qed.  
+    
+Lemma CoqType_to_camlType'_Rel mind ind Hparam Hfo larg T k : 
+let typ := (CoqType_to_camlType' (Σb := []) mind Hparam Hfo) in
+In larg (nth ind typ []) -> 
+nth_error larg k = Some T -> exists i, (k <= i) /\ (i < #| ind_bodies mind| + k) /\ T = Rel (i-k).
+Proof.
+  intro typ. destruct (nth_in_or_default ind typ []).
+  2: { rewrite e. intros Hlarg; destruct (in_nil Hlarg). }
+  intro Hlarg. unfold typ in *. eapply CoqType_to_camlType'_unfold in i.
+  destruct i as [ind' [Hfo' i]]. rewrite i in Hlarg. now eapply CoqType_to_camlType_oneind_Rel.
+Qed.
+
+Lemma CoqType_to_camlType'_Rel' mind ind Hparam Hfo larg T k : 
+let typ := (CoqType_to_camlType' (Σb := []) mind Hparam Hfo) in
+In larg (nth ind typ []) -> 
+nth_error larg k = Some T -> exists i, (0 <= i) /\ (i < #| ind_bodies mind|) /\ T = Rel i.
+Proof.
+  intros. unshelve epose (CoqType_to_camlType'_Rel _ ind); eauto. 
+  edestruct e as [i [? [? ?]]]; eauto. exists (i - k). repeat split; eauto.
+  all: lia.
+Qed.
+
+Inductive Forall2i {A B : Type} (R : nat -> A -> B -> Prop) (n : nat)
+  : list A -> list B -> Prop :=
+| Forall2i_nil : Forall2i R n [] []
+| Forall2i_cons :
+    forall x y l r,
+      R n x y ->
+      Forall2i R (S n) l r ->
+      Forall2i R n (x :: l) (y :: r).
+Arguments Forall2i_nil {_ _ _ _}.
+Arguments Forall2i_cons {_ _ _ _ _ _ _ _}.
+
+Derive Signature NoConfusionHom for All2i.
+
+Lemma Forall2_Forall_mix {A B} {P : B -> Prop} {Q : A -> B -> Prop}
+   {l : list A} {l' : list B} :
+  Forall2 (fun x y => (P y -> Q x y)) l l' -> Forall P l' -> Forall2 Q l l'.
+Proof.
+  induction 1; simpl; intros; constructor; inversion H1; eauto. 
+Qed.
+
+  Lemma Forall2_and_inv {A B : Type} (R R' : A -> B -> Prop) (l : list A) (l' : list B) :
+    Forall2 (fun (x : A) (y : B) => R x y /\ R' x y) l l'
+    -> Forall2 R l l' /\ Forall2 R' l l'.
   Proof.
-    intros adt Emind Σ Hflag Hind Hlookup [step Hrel].
-    revert v kn mind Hparam Hnparam Hfo ind adt Emind Eind Σ Hflag Hind Hlookup Hrel. 
+    induction 1; split; eauto; econstructor; destruct H; now destruct IHForall2.
+  Qed.
+
+  Definition camlValue_to_CoqValue_nil `{Heap} `{WcbvFlags} (cf:=config.extraction_checker_flags)
+    univ retro univ_decl kn mind
+    (Hparam : ind_params mind = [])
+    (Hindices : Forall (fun ind => ind_indices ind = []) (ind_bodies mind))
+    (Hnparam : ind_npars mind = 0)
+    (Hmono : ind_universes mind = Monomorphic_ctx)
+    (Hfo : is_true (forallb (@firstorder_oneind [] mind) (ind_bodies mind))) :
+    let adt := CoqType_to_camlType mind Hparam Hfo in
+    let Σ := mk_global_env univ [(kn , InductiveDecl mind)] retro in
+    PCUICTyping.wf Σ ->
+    with_constructor_as_block = true ->
+    forall v ind Eind, 
+    ind < List.length (snd adt) ->
+    lookup_inductive Σ (mkInd kn ind) = Some (mind, Eind) ->
+    realize_ADT _ [] [] adt [] All_nil ind v ->
+    exists t, forall h,  
+    ∥ (Σ , univ_decl) ;;; [] |- t : tInd (mkInd kn ind) [] ∥ /\ 
+    eval _ [] (empty_locals _) h (compile_pipeline Σ.(declarations) t) h v.
+  Proof. 
+    rename H into HHeap; rename H0 into H. 
+    intros adt Σ wfΣ Hflag v ind Eind Hind Hlookup [step Hrel].
+    revert kn mind Hparam Hindices Hnparam Hmono Hfo v ind Eind adt Σ wfΣ Hflag Hind Hlookup Hrel. 
     induction step; intros;  [inversion Hrel|].
     apply leb_correct in Hind. simpl in Hrel, Hind. 
     unfold Nat.ltb in Hrel. rewrite Hind in Hrel.
@@ -599,55 +859,82 @@ ind_universes0 ind_variance0) x Hparam Hfo'); eauto.
     - apply Existsi_spec in Hrel as [k [Ts [Hk [HkS [Hrel HTs]]]]].
       cbn in HkS.
       destruct (filter_firstn' _ _ _ _ HkS) as [k' [Hk' [Hfilter Hwit]]].
-      eexists (EAst.tConstruct (mkInd kn ind) k' []); cbn; split.
-      + sq. 
-        pose (MCList.nth_error_spec (ind_bodies mind) ind).
+      destruct Hwit as [As [Ha [Ha' Ha'']]].
+      eexists (tConstruct (mkInd kn ind) k' []); cbn; split.
+      + pose (MCList.nth_error_spec (ind_bodies mind) ind).
         destruct n; cbn; intros.
         2: { apply leb_complete in Hind.
              rewrite CoqType_to_camlType'_length in Hind. lia. }    
         pose (MCList.nth_error_spec (ind_ctors x) k').
         destruct n; intros; eauto.
-        ++ econstructor 2; eauto. cbn. rewrite ReflectEq.eqb_refl.
-        unfold Emind. cbn. rewrite nth_error_map. 
-        rewrite e. cbn. rewrite nth_error_map. rewrite e0. cbn.
-        reflexivity.
-        cbn; rewrite Hnparam; cbn.
-        destruct Hwit as [a' [? [_ ?]]].
-        destruct a'; [|inversion H1].
-        assert (is_true (@firstorder_oneind Σb mind x)).
-        { clear -e Hfo; eapply forallb_nth_error in Hfo; erewrite e in Hfo; exact Hfo. }
-        unshelve erewrite CoqType_to_camlType'_nth in Hfilter; eauto.
-        unshelve erewrite CoqType_to_camlType'_nth_length in Hk'; eauto.
-        unshelve erewrite CoqType_to_camlType'_nth in H0; eauto.
-        unfold CoqType_to_camlType_oneind in H0.
-        destruct x. destruct MCProd.andb_and. destruct (a _).
-        apply CoqType_to_camlType_ind_ctors_nth in H0.
-        destruct H0 as [a0 [? [? ?]]].
-        cbn in *.
-        rewrite e0 in H0. inversion H0. destruct H5. clear H0.
-        cbn in *.   
-        apply f_equal with (f := @List.length _) in H3.
-        rewrite CoqType_to_camlType_ind_ctors_length in H3.
-        rewrite rev_length in H3. cbn in H3. rewrite app_length in H3.
-        rewrite cstr_arity_length. lia. 
-        ++ assert (is_true (@firstorder_oneind Σb mind x)). 
+        ++ 
+          unshelve epose proof (Htyp := type_Construct (Σ, univ_decl) [] (mkInd kn ind) k' [] mind x x0 _ _ _).
+          ** econstructor.
+          ** unfold declared_constructor, declared_inductive. now cbn.
+          ** unfold consistent_instance_ext, consistent_instance; cbn.
+             now rewrite Hmono.
+          ** 
+          assert (is_true (@firstorder_oneind [] mind x)).
+          { clear -e Hfo; eapply forallb_nth_error in Hfo; erewrite e in Hfo; exact Hfo. }
+          unshelve erewrite CoqType_to_camlType'_nth in Hfilter, Ha, Ha'; eauto.
+          unfold CoqType_to_camlType_oneind in Hfilter, Ha, Ha'. destruct x. cbn in *. 
+          destruct MCProd.andb_and. destruct (a _).
+          apply CoqType_to_camlType_ind_ctors_nth in Ha.
+          destruct Ha as [a0 [? [? ?]]].
+          rewrite H2 in Ha''.
+          unfold type_of_constructor in Htyp.  
+          assert (CoqType_to_camlType_ind_ctor 0 #|ind_bodies mind|
+          (rev (cstr_args a0 ++ ind_params mind)) x = []).
+          { destruct CoqType_to_camlType_ind_ctor; eauto. }
+          clear Ha''. apply f_equal with (f := @List.length _) in H3.
+          rewrite CoqType_to_camlType_ind_ctors_length in H3.
+          cbn in H3. erewrite rev_length, app_length in H3.
+          assert (Ha0 : #|cstr_args a0| = 0) by lia. apply length_nil in Ha0.
+          rewrite e0 in H1. inversion H1. subst; clear H1.
+          unfold PCUICTyping.wf in wfΣ. inversion wfΣ as [_ wfΣ'].
+          cbn in wfΣ'. inversion wfΣ'; subst. clear X.
+          inversion X0 as [_ ? _ wf_ind]; cbn in *.
+          destruct wf_ind as [wf_ind _ _ _].
+          inversion wfΣ'; subst. inversion X1; subst. inversion on_global_decl_d. 
+            eapply Alli_nth_error in onInductives; eauto. cbn in onInductives.
+            inversion onInductives. unfold PCUICGlobalMaps.on_constructors in *. cbn in *.
+            eapply All2_nth_error_Some  in onConstructors; eauto. destruct onConstructors as [l' [? onConstructor]].
+          erewrite @cstr_eq with (i:=ind) in Htyp; eauto.
+          unfold cstr_concl in Htyp. 
+          erewrite Hparam, Ha0 in Htyp. cbn in Htyp. 
+          assert (cstr_indices a0 = []).
+          { apply length_nil. erewrite @cstr_indices_length with (Σ:=Σ) (ind:=(mkInd kn ind,k')); eauto. 
+            2: { repeat split. cbn. left. reflexivity. all:cbn; eauto. } cbn. eapply nth_error_forall in Hindices; eauto.
+                 cbn in Hindices. now rewrite Hindices. }
+          rewrite H1 in Htyp; clear H1; cbn in Htyp.
+          rewrite Ha0 Hparam in Htyp. cbn in Htyp.   
+          rewrite inds_spec in Htyp.  
+          assert (#|ind_bodies mind| - S ind + 0 + 0 - 0 = #|ind_bodies mind| - S ind)
+          by lia. rewrite H1 in Htyp; clear H1.
+          erewrite <- mapi_length in Htyp. 
+          rewrite <- nth_error_rev, nth_error_mapi, e in Htyp.
+          cbn in Htyp. sq; exact Htyp.  
+          now rewrite mapi_length.
+        ++ assert (is_true (@firstorder_oneind [] mind x)). 
         { clear -e Hfo; eapply forallb_nth_error in Hfo; erewrite e in Hfo; exact Hfo. }
           unshelve erewrite CoqType_to_camlType'_nth in Hk'; eauto.
           rewrite CoqType_to_camlType_oneind_length in Hk'.
-          lia.   
-      + rewrite compile_unfold_eq. simpl. 
+          lia.  
+     + rewrite (compile_pipeline_tConstruct_nil Σ). simpl. 
         unfold lookup_constructor_args. rewrite Hlookup.
         rewrite Hrel. clear Hrel v.
         pose (MCList.nth_error_spec (ind_bodies mind) ind).
         apply leb_complete in Hind. rewrite CoqType_to_camlType'_length in Hind.    
         destruct n; [|lia].
-        assert (is_true (@firstorder_oneind Σb mind x)).
+        assert (is_true (@firstorder_oneind [] mind x)).
         { clear -e Hfo; eapply forallb_nth_error in Hfo; erewrite e in Hfo; exact Hfo. }
-        unshelve erewrite CoqType_to_camlType'_nth in Hfilter; eauto.
-        cbn in Hlookup. rewrite ReflectEq.eqb_refl in Hlookup.
+        unshelve erewrite CoqType_to_camlType'_nth in Hfilter; eauto.  
+        unfold lookup_inductive, lookup_inductive_gen, lookup_minductive_gen in Hlookup. cbn in Hlookup.
+        rewrite ReflectEq.eqb_refl in Hlookup.
+        unfold nonblocks_until. 
         unshelve erewrite filter_length_nil with (mind:=mind) (ind:=ind); eauto.
-        2: { fold Emind. destruct (nth_error (EAst.ind_bodies Emind) ind); now inversion Hlookup. }
-        rewrite Hfilter.
+        2: { destruct (nth_error (ind_bodies mind) ind); now inversion Hlookup. }
+        rewrite Hfilter. 
         unshelve erewrite CoqType_to_camlType'_nth; eauto.
         unfold int_of_nat. set (Z.of_nat _).
         assert (z = (z mod Uint63.wB)%Z).
@@ -677,333 +964,487 @@ ind_universes0 ind_variance0) x Hparam Hfo'); eauto.
       destruct Ts as [|T Ts]. (* not possible filtered *) 
       + apply filter_nth_error in HTs. destruct HTs as [_ HTs]. 
         inversion HTs.
-      + pose proof (HTs':=HTs).
-        apply filter_nth_error in HTs. destruct HTs as [HTs _].
-        subst. inversion Hv'; subst.
-        cbn in H2.  
-        assert (Forall (fun v => (exists t : EAst.term,
-      ∥ EWcbvEval.value Σ t ∥ /\
-      eval CanonicalHeap []
-        (fun _ : Ident.t => not_evaluated)
-        empty_heap (compile Σ t) empty_heap v)) l').
-        { clear HTs' Hv' H2.
-          assert (exists l, incl Ts l /\ In l (nth ind (CoqType_to_camlType' mind Hparam Hfo) [])).
-          { exists (T::Ts). split; eauto. eapply incl_tl; apply incl_refl. }
-          clear HTs. rename H0 into HTs. 
-          induction H4; [eauto|].
-          econstructor; eauto.
-          { destruct x.
-          - destruct HTs as [? [? HTs]]. 
-            eapply CoqType_to_camlType'_fo_alt in HTs.
-            exfalso; apply HTs.
-            apply H1. econstructor 1. reflexivity.
-          - case_eq (n <? Datatypes.length
-          (CoqType_to_camlType' mind Hparam Hfo)); intro Heq. 
-          2: { apply Nat.leb_gt in Heq. cbn in H0. erewrite nth_overflow in H0.
-            inversion H0. rewrite to_list_length. lia. }
-          apply leb_complete in Heq. cbn in H0. 
-          rewrite to_list_nth in H0; [lia|].
-          pose (MCList.nth_error_spec (ind_bodies mind) ind).
-          rewrite CoqType_to_camlType'_length in Hind.    
-          destruct n0; [|lia].
-          pose (MCList.nth_error_spec (ind_bodies mind) n).
-          pose proof (Heq' := Heq). 
-          rewrite CoqType_to_camlType'_length in Heq.    
-          destruct n0; [|lia]. cbn.
-          eapply IHstep with (ind := n); eauto. 
-          eapply Heq'. cbn. rewrite ReflectEq.eqb_refl.
-          cbn. rewrite nth_error_map e0. cbn. reflexivity.
-          eauto.
-          - inversion H0. 
-          }
-          eapply IHForall2. destruct HTs as [? [? HTs]].
-          eexists; eauto. split; eauto.
-          intros a Ha. apply H1. econstructor 2; eauto.     
-        }
-        destruct (All_exists _ _ _ _ H0) as [lv' Hlv'].           
-        eapply Forall2_sym in Hlv'. 
+      + pose proof (HTs' := HTs). apply filter_nth_error in HTs. destruct HTs as [HTs _].
+        subst.
+        assert (Forall2 (fun v T => 
+        (exists t, forall h,  ∥ (Σ , univ_decl) ;;; [] |- fst t : tInd (mkInd kn (snd t)) [] ∥ /\ 
+        eval _ [] (empty_locals _) h (compile_pipeline Σ.(declarations) (fst t)) h v
+        /\ (0 <= snd t) /\ (snd t < #| ind_bodies mind|) /\ T = Rel (snd t))) v' (T::Ts)).
+        { 
+          assert (Forall (fun T => exists l l', In (l ++ [T] ++ l') (nth ind (CoqType_to_camlType' mind Hparam Hfo) [])) (T::Ts)).
+          { clear -HTs. set (l := T::Ts) in *. clearbody l.
+            assert (exists l', In (l' ++ l) (nth ind (CoqType_to_camlType' mind Hparam Hfo) [])).  
+            { exists []; eauto.  }
+            clear T Ts HTs; revert H. induction l; econstructor.
+            - destruct H as [l' HIn]. exists l'; exists l; eauto.
+            - eapply IHl. destruct H as [l' HIn]. exists (l' ++ [a]). 
+              now rewrite <- app_assoc. } 
+          eapply Forall2_Forall_mix; [| apply H0]; clear H0 Hwit HkS Hk HTs HTs'. 
+          unfold realize_value, to_realize_value in Hv'.
+          induction Hv'; econstructor. 
+          - clear IHHv'. intros [l0 [l0' HTs]].
+            unshelve eapply CoqType_to_camlType'_Rel with (k:=#|l0|) in HTs; try reflexivity.
+            3: { rewrite nth_error_app2; eauto. rewrite Nat.sub_diag. reflexivity. }
+            destruct HTs as [i [? [? Hx ]]]; subst. 
+            cbn in H0. unfold realize_term in H0.
+            destruct H0 as [t [h [h' [Hheap ?]]]].
+            specialize (H0 h h' _ Hheap). rewrite to_list_nth in H0.
+            + rewrite CoqType_to_camlType'_length. lia.
+            + pose (MCList.nth_error_spec (ind_bodies mind) (i - #|l0|)).
+              destruct n. 2: { clear -H1 H2 l1. lia. }
+              eapply IHstep in H0; eauto.
+              2: { unfold CoqType_to_camlType; cbn. now rewrite CoqType_to_camlType'_length. }
+              destruct H0 as [t' H0]. cbn. 
+              exists (t',i - #|l0|). intros. specialize (H0 h0). 
+              now cbn in *.
+              unfold lookup_inductive, lookup_inductive_gen, lookup_minductive_gen, lookup_env. cbn.
+              rewrite ReflectEq.eqb_refl. rewrite e; eauto.
+          - eapply IHHv'. }
+        pose proof (Hv'Ts := Forall2_length H0).
+        destruct (All_exists _ _ _ _ _ _ H0) as [lv' Hlv']. clear H0. 
+        eapply Forall2_sym in Hlv'. cbn in Hlv'.
+        pose proof (Forall2_forall _ _ Hlv'). clear Hlv'. rename H0 into Hlv'. 
+        eexists (mkApps (tConstruct (mkInd kn ind) k' []) (map fst lv')).
+        intro h. specialize (Hlv' h).  
         eapply Forall_Forall2_and_inv in Hlv'.
         destruct Hlv' as [Hlv' Hvallv'].
         apply Forall_All in Hvallv'.
-        apply All_sq in Hvallv'. destruct Hvallv'.
-        destruct T.
-        (* not first-order *)
-        * eapply CoqType_to_camlType'_fo_alt in HTs.
-          exfalso; apply HTs. econstructor 1; eauto. 
-        * case_eq (n <? Datatypes.length
-          (CoqType_to_camlType' mind Hparam Hfo)); intro Heq. 
-          2: { apply Nat.leb_gt in Heq. cbn in H2. erewrite nth_overflow in H2.
-            inversion H2. rewrite to_list_length. lia. }
-          apply leb_complete in Heq. cbn in H2. 
-          rewrite to_list_nth in H2; [lia|].
-          pose (MCList.nth_error_spec (ind_bodies mind) ind).
-          rewrite CoqType_to_camlType'_length in Hind.    
-          destruct n0; [|lia].
-          pose (MCList.nth_error_spec (ind_bodies mind) n).
-          pose proof (Heq' := Heq). 
-          rewrite CoqType_to_camlType'_length in Heq.    
-          destruct n0; [|lia]. cbn. 
-          eapply IHstep with (kn:=kn) in H2; eauto; cbn.  
-          destruct H2 as [vy [? Hvy]]. 
-          eexists (EAst.tConstruct (mkInd kn ind) k' (vy :: lv')); cbn; split.
-          2: { rewrite compile_unfold_eq. simpl. 
-          unfold lookup_constructor_args. rewrite Hlookup.
-          assert (is_true (@firstorder_oneind Σb mind x)).
-          { clear -e Hfo; eapply forallb_nth_error in Hfo; erewrite e in Hfo; exact Hfo. }
-          assert (is_true (@firstorder_oneind Σb mind x0)).
-          { clear -e0 Hfo. eapply forallb_nth_error in Hfo; erewrite e0 in Hfo. exact Hfo. }
+          split.
+          2: { rewrite (compile_pipeline_tConstruct_cons Σ). 
+            rewrite map_length. erewrite Forall2_length; eauto.
+            pose proof (Forall2_length Hv').
+            rewrite zip_length; try rewrite <- H0; cbn; lia.
+            unfold lookup_constructor_args. rewrite Hlookup.
+            unfold lookup_inductive, lookup_inductive_gen, lookup_minductive_gen in Hlookup.
+            cbn in Hlookup. rewrite ReflectEq.eqb_refl in Hlookup.
+            assert (HEind : nth_error (ind_bodies mind) ind = Some Eind).
+            { destruct (nth_error (ind_bodies mind) ind); now inversion Hlookup. }          
+          assert (is_true (@firstorder_oneind [] mind Eind)).
+          { clear - HEind Hfo; eapply forallb_nth_error with (n := ind) in Hfo.
+            rewrite HEind in Hfo. exact Hfo. }
           unshelve erewrite CoqType_to_camlType'_nth; try eapply e; eauto.
-          cbn in Hlookup. rewrite ReflectEq.eqb_refl in Hlookup.
+          2: { rewrite CoqType_to_camlType'_length in Hind. lia. }
+          unfold blocks_until.
           unshelve erewrite filter_length_not_nil with (mind:=mind) (ind:=ind); eauto.
-          2: { fold Emind. destruct (nth_error (EAst.ind_bodies Emind) ind); now inversion Hlookup. }
           unshelve erewrite CoqType_to_camlType'_nth; try eapply e; eauto.
+          2: { rewrite CoqType_to_camlType'_length in Hind. lia. }                  
           econstructor.
-          - econstructor.
-            + exact Hvy.
-            + apply Forall2_acc_cst. 
-              rewrite MCList.map_InP_spec.
-              rewrite <- (map_id l'). apply Forall2_map. 
-              exact Hlv'.
-          - cbn. apply Forall2_length in H4. rewrite <- H4.
-          assert (is_true (@firstorder_oneind Σb mind x)).
-          { clear -e Hfo; eapply forallb_nth_error in Hfo; erewrite e in Hfo; exact Hfo. }
-          unshelve erewrite CoqType_to_camlType'_nth with (x:=x) in HTs ; eauto.  
-          unfold CoqType_to_camlType_oneind in HTs.
-          destruct x, MCProd.andb_and, (a _).
-          apply In_nth_error in HTs.
-          destruct HTs as [j HTs].
-          apply CoqType_to_camlType_ind_ctors_nth in HTs.
-          destruct HTs as [? [? [? HTs]]].
-          apply f_equal with (f := @List.length _) in HTs. 
-          rewrite CoqType_to_camlType_ind_ctors_length in HTs.
-          cbn in HTs. rewrite Hparam in HTs.
-          rewrite rev_length app_length in HTs. cbn in HTs.    
-          rewrite HTs. rewrite <- plus_n_O.
-          unshelve eapply ctors_max_length; try eapply e; eauto.
+          - apply Forall2_acc_cst. 
+            rewrite MCList.map_InP_spec.
+            rewrite <- (map_id v'). apply Forall2_map. 
+            rewrite Forall2_map_left. 
+            eapply Forall2_and_inv in Hlv'. destruct Hlv' as [Hlv' _].
+            erewrite <- (Forall2_map_right (fun a b =>
+            eval HHeap [] (empty_locals HHeap) h
+              (compile_pipeline [(kn, InductiveDecl mind)]
+                 (fst a)) h b) fst) in Hlv'.
+            rewrite zip_fst in Hlv'; eauto. 
+          - cbn. erewrite <- Forall2_length; eauto.
+            clear Hlv'. eapply In_nth_error in HTs.
+            destruct HTs as [k HTs]. pose proof (HEind' := HEind).
+            unshelve erewrite CoqType_to_camlType'_nth in HTs; eauto.
+            2: { rewrite CoqType_to_camlType'_length in Hind. lia. }                  
+            eapply CoqType_to_camlType_oneind_nth in HTs.
+            destruct HTs as [l' [HTs Hlength]].
+            rewrite Hlength. eapply ctors_max_length; eauto.
           }
-          2: { cbn. rewrite ReflectEq.eqb_refl.
-          unfold ErasureFunction.erase_mutual_inductive_body.
-          rewrite nth_error_map e0. reflexivity. }
-          pose (MCList.nth_error_spec (ind_ctors x) k').
-          destruct n0; intros; eauto.
-          ++ sq. econstructor 2; eauto. cbn.
-          rewrite ReflectEq.eqb_refl.
-          unfold Emind. cbn. rewrite nth_error_map. 
-          rewrite e. cbn. rewrite nth_error_map. rewrite e1. cbn.
-          reflexivity.
-          cbn; rewrite Hnparam; cbn.
-          destruct Hwit as [a' [? [? ?]]].
-          assert (is_true (@firstorder_oneind Σb mind x)).
-          { clear -e Hfo; eapply forallb_nth_error in Hfo; erewrite e in Hfo; exact Hfo. }
-          apply Forall2_length in Hlv'. rewrite Hlv'.
-          apply Forall2_length in Hv'. cbn in Hv'.
-          inversion Hv'.
-          rewrite Nat.sub_0_r in HTs'. rewrite H3 in HTs'.    
-          unshelve erewrite CoqType_to_camlType'_nth with (x:=x) in H2; eauto.
-          unfold CoqType_to_camlType_oneind in H2.
-          destruct x. destruct MCProd.andb_and. destruct (a _).
-          apply CoqType_to_camlType_ind_ctors_nth in H2.
-          destruct H2 as [a0 [? [? ?]]].
-          cbn in *.
-          rewrite e1 in H2. inversion H2. destruct H10. clear H2.
-          cbn in *.
-          rewrite cstr_arity_length.
-          apply f_equal with (f := @List.length _) in H7.
-          rewrite CoqType_to_camlType_ind_ctors_length in H7.
-          rewrite rev_length in H7. cbn in H3. rewrite app_length in H7.
-          rewrite Hparam in H7. cbn in H7. rewrite <- plus_n_O in H7.
-          rewrite <- H7. now inversion HTs'.
-          ++ assert (is_true (@firstorder_oneind Σb mind x)). 
-        { clear -e Hfo; eapply forallb_nth_error in Hfo; erewrite e in Hfo; exact Hfo. }
-          unshelve erewrite CoqType_to_camlType'_nth with (x:=x) in Hk'; eauto.
-          rewrite CoqType_to_camlType_oneind_length in Hk'.
-          lia. 
-        * inversion H2.  
-  Qed.
+        clear Hv'. 
+        destruct Hwit as [Ts' [HTs'' [Hfilter _]]].
+        unfold lookup_inductive, lookup_inductive_gen, lookup_minductive_gen in Hlookup.
+        unfold lookup_inductive, lookup_inductive_gen, lookup_minductive_gen in Hlookup.
+        cbn in Hlookup. rewrite ReflectEq.eqb_refl in Hlookup.
+        assert (HEind : nth_error (ind_bodies mind) ind = Some Eind).
+        { destruct (nth_error (ind_bodies mind) ind); now inversion Hlookup. }
+        assert (is_true (@firstorder_oneind [] mind Eind)).
+        { clear - HEind Hfo; eapply forallb_nth_error in Hfo; erewrite HEind in Hfo; exact Hfo. }
+        unshelve erewrite CoqType_to_camlType'_nth in Hfilter, HTs,HTs', HTs''; eauto.
+          2-5 : rewrite CoqType_to_camlType'_length in Hind; lia.
+          unfold CoqType_to_camlType_oneind in Hfilter, HTs, HTs', HTs''. remember Eind as o. destruct o. 
+          destruct MCProd.andb_and. destruct (a _).  
+          apply CoqType_to_camlType_ind_ctors_nth in HTs''.
+          destruct HTs'' as [a0 [? [? ?]]]. rewrite Nat.sub_0_r in HTs'. rewrite HTs' in Hfilter. 
+          inversion Hfilter. clear HTs HTs' Hfilter. rewrite H4 in Hlv', Hv'Ts. clear T Ts H4.   
+          eapply Forall2_and_inv in Hlv'. destruct Hlv' as [_ Hlv'].
+          set (P := (fun a b =>
+          0 <= a /\ a < #|ind_bodies mind| /\ b = Rel a)). 
+          epose proof (Forall2_map_right (fun a => P (snd a)) snd). unfold P in H3.
+          rewrite <- H3 in Hlv'. clear H3.
+          epose proof (Forall2_map_left P snd). unfold P in H3.
+          rewrite <- H3 in Hlv'. clear H3 P. 
+          rewrite zip_snd in Hlv'; eauto. 
+          eapply Forall2_All2 in Hlv'.
+          assert (Hcstr_indices : cstr_indices a0 = []).
+          { apply length_nil. erewrite @cstr_indices_length with (Σ:=Σ) (ind:=(mkInd kn ind,k')); eauto. 
+            2: { repeat split. cbn. left. reflexivity. all:cbn; eauto. } cbn. eapply nth_error_forall in Hindices; eauto.
+                 cbn in Hindices. now rewrite Hindices. }
+          sq. eapply PCUICGeneration.type_mkApps.
+          ++ eapply type_Construct; eauto. 
+          ** unfold declared_constructor, declared_inductive. now cbn.
+          ** unfold consistent_instance_ext, consistent_instance; cbn.
+             now rewrite Hmono. 
+          ++ unfold PCUICTyping.wf in wfΣ. inversion wfΣ as [_ wfΣ'].
+            cbn in wfΣ'. inversion wfΣ'. clear X. inversion X0. inversion on_global_decl_d. 
+            eapply Alli_nth_error in onInductives; eauto. cbn in onInductives.
+            inversion onInductives. unfold PCUICGlobalMaps.on_constructors in *. cbn in *.
+            unfold type_of_constructor. cbn.
+            eapply All2_nth_error_Some  in onConstructors; eauto. destruct onConstructors as [l' [? onConstructor]].
+            erewrite cstr_eq; eauto. 
+            revert Hlv'. induction Hvallv'; cbn; intro Hlv'.
+            ** inversion Hlv'. destruct a0, cstr_args0.
+            2:{ subst. cbn in *. set (CoqType_to_camlType_ind_ctor _ _ _ x) in H7.
+                assert (#|[]| = #|l|) by now f_equal.
+                unfold l in H2. rewrite CoqType_to_camlType_ind_ctors_length in H2.
+                rewrite app_length in H2. cbn in H2. clear -H2; lia. }
+                rewrite Hparam. cbn. unfold cstr_concl, cstr_concl_head; cbn.
+                cbn in Hcstr_indices. rewrite Hparam; cbn. rewrite Hcstr_indices.
+                cbn. rewrite nth_error_inds. 
+                { clear -Hlookup. destruct (ind_bodies mind); cbn in *; try lia.
+                rewrite nth_error_nil in Hlookup. inversion Hlookup. }
+                assert (#|ind_bodies mind| - S (#|ind_bodies mind| - S ind + 0 + 0 - 0) = ind).
+                { rewrite CoqType_to_camlType'_length in Hind. clear - Hind. lia. }
+                rewrite H3; clear H3. cbn. econstructor; try reflexivity.          
+            unfold isType, PCUICEnvTyping.infer_sort. exists ind_sort0.
+            rewrite Hparam in ind_arity_eq. cbn in ind_arity_eq.
+            eapply nth_error_forall in Hindices; eauto. cbn in Hindices. rewrite Hindices in ind_arity_eq.                       
+            cbn in ind_arity_eq.  
+            unshelve epose proof (type_Ind (Σ,univ_decl) [] (mkInd kn ind) [] mind Eind _ _ _).
+            *** econstructor.
+            *** unfold declared_constructor, declared_inductive. subst. now cbn.
+            *** unfold consistent_instance_ext, consistent_instance; cbn.
+               now rewrite Hmono.
+            *** subst. cbn in *. destruct ind_sort0; eauto. cbn in X.
+                admit. 
+          **  destruct a0, cstr_args0; subst; cbn in *. 
+           { eapply All2_length in Hlv'. rewrite CoqType_to_camlType_ind_ctors_length in Hlv'.
+           rewrite Hparam in Hlv'. inversion Hlv'. }
+           rewrite Hparam. cbn. unfold cstr_concl, cstr_concl_head; cbn.
+           admit. 
+  Admitted.
   
-  From Malfunction Require Import CompileCorrect.
+  Definition CoqValue_to_CamlValue `{Heap} `{WcbvFlags} (cf:=config.extraction_checker_flags)
+    univ retro univ_decl kn mind
+    (Hparam : ind_params mind = [])
+    (Hindices : Forall (fun ind => ind_indices ind = []) (ind_bodies mind))
+    (Hnparam : ind_npars mind = 0)
+    (Hmono : ind_universes mind = Monomorphic_ctx)
+    (Hfo : is_true (forallb (@firstorder_oneind [] mind) (ind_bodies mind))) :
+    let adt := CoqType_to_camlType mind Hparam Hfo in
+    let Σ := mk_global_env univ [(kn , InductiveDecl mind)] retro in
+    PCUICTyping.wf Σ ->
+    with_constructor_as_block = true ->
+    forall t ind Eind, 
+    ind < List.length (snd adt) ->
+    lookup_inductive Σ (mkInd kn ind) = Some (mind, Eind) ->
+    ∥ (Σ , univ_decl) ;;; [] |- t : tInd (mkInd kn ind) [] ∥ ->
+    forall h v, 
+      eval _ [] (empty_locals _) h (compile_pipeline Σ.(declarations) t) h v
+      -> realize_ADT _ [] [] adt [] All_nil ind v.
+  Proof.
+  Admitted.  
 
-  Definition CoqValue_to_CamlValue `{WcbvFlags} 
-  (cf:=config.extraction_checker_flags) {guard : abstract_guard_impl}
-  (Σ:reference_impl_ext) kn mind Eind 
-  {normal_in : forall Σ_ : global_env_ext,
-  wf_ext Σ_ -> Σ_ ∼_ext Σ -> PCUICSN.NormalizationIn Σ_}
-(retro : Retroknowledge.t)
-(Hparam : ind_params mind = [])
-(Hnparam : ind_npars mind = 0)
-(Hfo : is_true (forallb (@firstorder_oneind Σb mind) (ind_bodies mind))) ind univ v u t vErase' :
-let adt := CoqType_to_camlType mind Hparam Hfo in
-let Emind := ErasureFunction.erase_mutual_inductive_body mind in 
-let Σ' := [(kn , EAst.InductiveDecl Emind)] in
-let global_adt := add_ADT CanonicalHeap [] [] kn adt in 
-Σ.(reference_impl_env_ext) = (mk_global_env univ [(kn , InductiveDecl mind)] retro ,Monomorphic_ctx) ->
-with_constructor_as_block = true ->
-ind < List.length (snd adt) ->
-EGlobalEnv.lookup_inductive Σ' (mkInd kn ind) = Some (Emind, Eind) ->
-forall (wt : Σ ;;; [] |- t : tInd (mkInd kn ind) u)
-(wv : Σ ;;; [] |- v : tInd (mkInd kn ind) u),  
-let tErase := ErasureFunction.erase (normalization_in := normal_in) canonical_abstract_env_impl Σ [] t 
-(fun Σ' e => match (eq_sym e) in (_ = ΣΣ) return welltyped ΣΣ [] t with eq_refl => iswelltyped wt end) in 
-let vErase := ErasureFunction.erase (normalization_in := normal_in) canonical_abstract_env_impl Σ [] v 
-(fun Σ' e => match (eq_sym e) in (_ = ΣΣ) return welltyped ΣΣ [] v with eq_refl => iswelltyped wv end) in 
-PCUICWcbvEval.eval Σ t v ->
-EWcbvEval.eval Σ' tErase vErase ->
-represents_value vErase' vErase ->
-eval [] (fun _ => not_evaluated) empty_heap
-    (compile Σ' tErase)
-    empty_heap (compile_value Σ' vErase') ->
-realize_val CanonicalHeap [] []
-            global_adt (Adt kn (int_of_nat ind) []) (compile_value Σ' vErase').
+  From Malfunction Require Import CompileCorrect Pipeline.
+
+  Section fix_global.
+
+  Variable Σ : list Ident.t.
+
+  Fixpoint isPure (t : t) :=
+    match t with
+    | Mvar x => true
+    | Mlambda (ids, x) => isPure x
+    | Mapply (x, args) => isPure x && forallb isPure args
+    | Mlet (binds, x) => forallb isPure_binding binds && isPure x
+    | Mnum x => true
+    | Mstring x => false (* strings are interpreted using vectors *)
+    | Mglobal id => true
+    | Mswitch (x, sels) => isPure x && forallb (fun '(_, x) => isPure x) sels
+    | Mnumop1 (op, num, x) => isPure x
+    | Mnumop2 (op, num, x1, x2) => isPure x1 && isPure x2
+    | Mconvert (from, to, x) => isPure x
+    | Mblock (tag, xs) => forallb isPure xs
+    | Mfield (i, x) => isPure x
+    | _ => false
+    end
+  with isPure_binding (b : binding) :=
+         match b with
+         | Unnamed x => isPure x
+         | Named (id, x) => isPure x
+         | Recursive recs => forallb (fun '(id,x) => isPure x) recs
+         end.
+
+  Definition isPure_rec_value `{Heap} (v : rec_value) :=
+    match v with 
+    | RFunc (_ , t) => is_true (isPure t)
+    | Bad_recursive_value => True
+    | _ => False
+    end. 
+
+  Fixpoint isPure_value `{Heap} (v : value) {struct v} :=
+    match v with
+    | Block (_,vs) => Forall (fun p => p) (map isPure_value vs)
+    | Func (locals,_,t) => (forall s, isPure_value (locals s)) /\ is_true (isPure t)    
+    | RClos (locals,self,mfix,t) => (forall s, isPure_value (locals s)) /\ Forall isPure_rec_value mfix
+    | value_Int _ => True
+    | Float _ => True
+    | fail _ => True
+    | _ => False
+    end.
+
+End fix_global.
+
+Lemma isPure_add_self `{Heap} locals mfix self s :
+  (forall s : Ident.t, isPure_value (locals s)) ->
+  Forall isPure_rec_value mfix ->
+  isPure_value (add_self self mfix locals s).
 Proof.
-  intros. cbn. rewrite ReflectEq.eqb_refl.
-  rewrite int_to_of_nat. admit.
-  pose proof (X':=X).
-  eapply @PCUICClassification.eval_classification with (args := []) in X; eauto.
-  destruct v; try solve [inversion X]; cbn in X.   
-  admit.
-  (*cbn in vErase.
-  admit. 
-  induction vErase'.      
-  3: { destruct args; unfold compile_value. unfold lookup_constructor_args.
-       cbn.  ErasureFunction.erase_correct_firstorder } 
-    EWcbvEval.eval
-  EWcbvEvalNamed.eval Σ Γ s t
-  SemanticsSpec.eval Σ' Γ' h (compile Σ s) h (compile_value Σ t).
-*)
-Abort.
-  Definition CoqFunction_to_CamlFunction `{WcbvFlags} 
-    (cf:=config.extraction_checker_flags) {guard : abstract_guard_impl}
-    (Σ:reference_impl_ext) kn mind Eind 
-    {normal_in : forall Σ_ : global_env_ext,
-    wf_ext Σ_ -> Σ_ ∼_ext Σ -> PCUICSN.NormalizationIn Σ_}
-  (retro : Retroknowledge.t)
+  intros Hlocals Hmfix. unfold add_self, add_recs, List.mapi.
+  generalize 0 as i. generalize self at 1. 
+  induction self; cbn; eauto.
+  unfold Ident.Map.add. destruct (Ident.eqb s a); cbn; eauto.
+Qed.
+
+Lemma isPure_heap `{Heap} `{WcbvFlags} locals h h' t v :
+  is_true (isPure t) ->
+  (forall s, isPure_value (locals s)) -> 
+  eval [] locals h t h' v -> isPure_value v /\ h = h'.
+Proof.
+  intros Hpure Hlocals. induction 1; try solve [inversion Hpure]; cbn in Hpure;
+  repeat rewrite MCProd.andb_and in Hpure; try solve [cbn; repeat split; eauto]; eauto. 
+  - cbn in *. destruct Hpure as [? [? ?]].
+    try (destruct IHeval1; eauto);
+     try (destruct IHeval2; eauto); try (destruct IHeval3; eauto); try now eauto.
+    destruct H4. intros s. unfold Ident.Map.add. destruct (Ident.eqb s x); eauto.
+  - destruct Hpure as [? [? ?]].
+    try (destruct IHeval1; eauto);
+     try (destruct IHeval2; eauto); try (destruct IHeval3; eauto); try now eauto.
+    destruct H5. pose proof (proj1 (Forall_nth _ _) H9 n Bad_recursive_value). rewrite H1 in H10.
+    eapply H10. case_eq (Nat.ltb n #|mfix|); try rewrite Nat.ltb_lt; eauto.
+    rewrite Nat.ltb_ge. intro neq.  rewrite nth_overflow in H1; eauto. inversion H1.  
+    destruct H5. intros s. unfold Ident.Map.add. destruct (Ident.eqb s y); eauto.
+    eapply isPure_add_self; eauto. 
+  - cbn in *. destruct Hpure as [? [? ?]]; try (destruct IHeval1; eauto); now eauto.
+  - destruct Hpure as [? [? [? ?]]]. repeat rewrite MCProd.andb_and in IHeval.
+    destruct IHeval ; eauto.
+  - cbn in *. destruct Hpure as [[? ?] ?]; try (destruct IHeval1; eauto); try (destruct IHeval2; eauto); now eauto.  
+  - cbn in *. destruct Hpure as [[? ?] ?]; try (destruct IHeval1; eauto); try (destruct IHeval2; eauto); try now eauto.
+    intros s. unfold Ident.Map.add. destruct (Ident.eqb s x); eauto.
+  - cbn in *. destruct Hpure as [[? ?] ?]; try (destruct IHeval; eauto); try now eauto.
+    intros s. rewrite H1. eapply isPure_add_self; eauto. unfold rfunc, RFunc_build.
+    eapply forallb_Forall in H3. clear -H3. induction recs; eauto; cbn. destruct a; cbn in *. inversion H3; subst.
+    econstructor; eauto. destruct t0; cbn; eauto. destruct p. cbn in H2. destruct l; cbn ; eauto.
+    destruct l; cbn ; eauto.
+  - cbn in *. destruct Hpure as [? ?]; try (destruct IHeval1; eauto); try (destruct IHeval2; eauto); try now eauto.
+    induction cases; cbn in *. inversion H1. repeat rewrite MCProd.andb_and in H3. destruct H3.   
+    destruct a. destruct (existsb _ _); [inversion H1; subst; eauto|]. now eapply IHcases.
+  - cbn in *. clear H1 H2. induction H3; [now eauto|]. repeat rewrite MCProd.andb_and in Hpure.
+    destruct Hpure. destruct IHForall2_acc; eauto. destruct H1; eauto. cbn; split; now eauto.
+  - cbn in *. destruct IHeval; eauto. split; eauto. eapply Forall_nth; eauto. now eapply Forall_map_inv in H4.
+  - cbn in *. now eauto.
+  - cbn in *. inversion H1.
+  - cbn in *. destruct IHeval; eauto.
+  - cbn. destruct Hpure. destruct IHeval1; eauto. destruct IHeval2; eauto. now destruct op.
+  - cbn; now eauto.   
+  - cbn; destruct Hpure. destruct IHeval1; eauto. destruct IHeval2; now eauto.
+  - cbn; destruct Hpure. destruct IHeval1; eauto. destruct IHeval2; now eauto.
+  - cbn; destruct IHeval; eauto. 
+  - cbn. destruct IHeval; eauto.
+  - cbn. destruct IHeval; eauto.
+Qed.            
+
+Lemma isPure_heap_irr `{Heap} `{WcbvFlags} h h' locals t v :
+  is_true (isPure t) ->
+  (forall s, isPure_value (locals s)) -> 
+  eval [] locals h t h' v -> forall h'', eval [] locals h'' t h'' v.
+Proof.
+  intros Hpure Hlocals. induction 1; try solve [inversion Hpure]; cbn in Hpure;
+  repeat rewrite MCProd.andb_and in Hpure; try solve [cbn; destruct Hpure; econstructor; eauto]; 
+  try solve [cbn; econstructor; eauto].
+  - intro. destruct Hpure as [? [? ?]]. econstructor 3; eauto.
+    eapply isPure_heap in H1_, H1_0; eauto. destruct H1_ as [[Hlocals' He] _].  
+    eapply IHeval3; eauto. intros s. unfold Ident.Map.add. destruct (Ident.eqb s x); now eauto.
+  - intro. destruct Hpure as [? [? ?]]. econstructor 4; eauto.
+    eapply isPure_heap in H1_, H1_0; eauto. destruct H1_ as [[Hlocals' He] _].
+    pose proof (proj1 (Forall_nth _ _) He n Bad_recursive_value).
+    rewrite H1 in H5. cbn in H5. eapply IHeval3.
+    case_eq (Nat.ltb n #|mfix|); try rewrite Nat.ltb_lt; eauto.
+    rewrite Nat.ltb_ge. intro neq. rewrite nth_overflow in H1; eauto. inversion H1.  
+    destruct H1_0. intros s. unfold Ident.Map.add. destruct (Ident.eqb s y); eauto.
+    eapply isPure_add_self; eauto. 
+  - intro. destruct Hpure as [? [? ?]]. econstructor 6; eauto.
+    eapply IHeval; eauto. cbn. now repeat rewrite MCProd.andb_and.
+  - intro. destruct Hpure as [[? ?] ?]. econstructor; eauto. eapply IHeval2; eauto. 
+    cbn. now repeat rewrite MCProd.andb_and.
+  - intro. destruct Hpure as [[? ?] ?]. econstructor; eauto. eapply IHeval2; eauto. 
+    cbn. now repeat rewrite MCProd.andb_and. 
+    intros s. unfold Ident.Map.add. destruct (Ident.eqb s x); eauto. eapply isPure_heap in H1_; now eauto. 
+  - intro. destruct Hpure as [[? ?] ?]. econstructor; eauto. rewrite H1 in IHeval. eapply IHeval; eauto; cbn.
+    now repeat rewrite MCProd.andb_and. intro s. eapply isPure_add_self; eauto.
+    unfold rfunc, RFunc_build.
+    eapply forallb_Forall in H3. clear -H3. induction recs; eauto; cbn. destruct a; cbn in *. inversion H3; subst.
+    econstructor; eauto. destruct t0; cbn; eauto. destruct p. cbn in H2. destruct l; cbn ; eauto.
+    destruct l; cbn ; eauto. 
+  - destruct Hpure. econstructor; eauto. eapply IHeval2; eauto.   
+    induction cases; cbn in *. inversion H1. repeat rewrite MCProd.andb_and in H3. destruct H3.   
+    destruct a. destruct (existsb _ _); [inversion H1; subst; eauto|]. now eapply IHcases.
+  - econstructor; eauto. clear H1 H2. induction H3; [econstructor; eauto|].
+    cbn in Hpure. rewrite MCProd.andb_and in Hpure. destruct Hpure. econstructor; eauto.
+Qed. 
+
+(* Definition extract `{Heap} := Transform.run verified_malfunction_pipeline.*)
+
+Lemma compile_pure `{Heap} `{WcbvFlags} Σ t : is_true (isPure (compile_pipeline Σ t)).
+Proof.
+Admitted.
+
+Definition compile_compose `{Heap} `{WcbvFlags} Σ h h' t u' u v w:
+  eval [] (empty_locals _) h (compile_pipeline Σ u) h v ->
+  eval [] (empty_locals _) h u' h' v ->
+  eval [] (empty_locals _) h (Mapply (compile_pipeline Σ t, [u'])) h' w ->
+  eval [] (empty_locals _) h (compile_pipeline Σ (tApp t u)) h w.
+Admitted. 
+
+Definition compile_function `{Heap} `{WcbvFlags} (cf:=config.extraction_checker_flags)
+  Σ univ_decl h h' f v na A B :
+  ∥ (Σ , univ_decl) ;;; [] |- f : tProd na A B ∥ ->
+  eval [] (empty_locals _) h (compile_pipeline Σ.(declarations) f) h' v ->
+  isFunction v = true.
+Admitted.
+
+Definition CoqFunction_to_CamlFunction `{Heap} `{WcbvFlags} (cf:=config.extraction_checker_flags)
+    univ retro univ_decl kn mind 
   (Hparam : ind_params mind = [])
+  (Hindices : Forall (fun ind => ind_indices ind = []) (ind_bodies mind))
   (Hnparam : ind_npars mind = 0)
-  (Hfo : is_true (forallb (@firstorder_oneind Σb mind) (ind_bodies mind))) ind univ v u f na:
+  (Hmono : ind_universes mind = Monomorphic_ctx)
+  (Hfo : is_true (forallb (@firstorder_oneind [] mind) (ind_bodies mind))) ind Eind f na:
   let adt := CoqType_to_camlType mind Hparam Hfo in
-  let Emind := ErasureFunction.erase_mutual_inductive_body mind in 
-  let Σ' := [(kn , EAst.InductiveDecl Emind)] in
-  let global_adt := add_ADT CanonicalHeap [] [] kn adt in 
-  Σ.(reference_impl_env_ext) = (mk_global_env univ [(kn , InductiveDecl mind)] retro ,Monomorphic_ctx) ->
+  let Σ := mk_global_env univ [(kn , InductiveDecl mind)] retro in
+  let global_adt := add_ADT _ [] [] kn adt in 
+  PCUICTyping.wf Σ ->
   with_constructor_as_block = true ->
   ind < List.length (snd adt) ->
-  EGlobalEnv.lookup_inductive Σ' (mkInd kn ind) = Some (Emind, Eind) ->
-  forall (wt : Σ ;;; [] |- f : tProd na (tInd (mkInd kn ind) u) (tInd (mkInd kn ind) u)),  
-  eval [] (fun _ => not_evaluated) empty_heap
-      ((compile Σ' (ErasureFunction.erase (normalization_in := normal_in) canonical_abstract_env_impl Σ [] f 
-          (fun Σ' e => match (eq_sym e) in (_ = ΣΣ) return welltyped ΣΣ [] f with eq_refl => iswelltyped wt end))))
-      empty_heap v ->
-  realize_val CanonicalHeap [] []
-              global_adt (Arrow (Adt kn (int_of_nat ind) []) (Adt kn (int_of_nat ind) [])) v.
+  lookup_inductive Σ (mkInd kn ind) = Some (mind, Eind) ->
+  ∥ (Σ , univ_decl) ;;; [] |- f : tProd na (tInd (mkInd kn ind) []) (tInd (mkInd kn ind) []) ∥ ->
+  realize_term _ [] []
+        global_adt (Arrow (Adt kn (int_of_nat ind) []) (Adt kn (int_of_nat ind) [])) 
+        (compile_pipeline Σ.(declarations)  f).
 Proof.
-  intros. cbn. rewrite ReflectEq.eqb_refl. cbn.
-
-  do 3 eexists. split; intros. 
-  2: {
-    rewrite int_to_of_nat; [admit|].
-    eapply camlValue_to_CoqValue_nil in H5; eauto; cbn.
-    2: { rewrite int_to_of_nat. admit. eauto. }
-    2: { rewrite ReflectEq.eqb_refl. rewrite int_to_of_nat. admit.
-        cbn. rewrite nth_error_map. admit. }
-    destruct H5 as [? [? ?]].
-         
-    }   
-
-    } 
-
-
-  Existing Instance config.extraction_checker_flags.
-
-
-
-  Definition camlValue_to_CoqValue_gen `{WcbvFlags}  
-    Σ kn mind Eind 
-    (Hparam : ind_params mind = [])
-    (Hnparam : ind_npars mind = 0)
-    (Hfo : is_true (forallb (@firstorder_oneind Σb mind) (ind_bodies mind))) ind v :
-    let adt := CoqType_to_camlType mind Hparam Hfo in
-    let Emind := ErasureFunction.erase_mutual_inductive_body mind in 
-    with_constructor_as_block = true ->
-    ind < List.length (snd adt) ->
-    EGlobalEnv.lookup_inductive Σ (mkInd kn ind) = Some (Emind, Eind) ->
-    realize_ADT CanonicalHeap [] [] adt [] All_nil ind v ->
-    exists t, ∥ EWcbvEval.value Σ t ∥ /\ 
-    eval CanonicalHeap [] (fun _ => not_evaluated) empty_heap (compile Σ t) empty_heap v.
-  Proof.
-    induction Σ; cbn; intros.
-    - cbn in H3. inversion H2.
-    - destruct a. cbn in *.     
-      destruct ReflectEq.eqb.
-      2: { eapply IHΣ. ; eauto.  }   
-
-  Definition camlValue_to_CoqValue `{WcbvFlags} Σ global_adt kn mind (Hparam : ind_params mind = [])
-      (Hfo : is_true (forallb (@firstorder_oneind Σb mind) (ind_bodies mind))) ind v :
-      let adt := CoqType_to_camlType mind Hparam Hfo in
-      let Emind := ErasureFunction.erase_mutual_inductive_body mind in 
-      let Σ' := (kn , EAst.InductiveDecl Emind) :: Σ in
-      with_constructor_as_block = false ->
-      ind < List.length (snd adt) ->
-      realize_ADT CanonicalHeap [] global_adt adt [] All_nil ind v ->
-      exists t, ∥ EWcbvEval.value Σ' t ∥ /\ 
-      eval CanonicalHeap [] (fun _ => not_evaluated) empty_heap (compile Σ' t) empty_heap v.
-    Proof.
-      revert v kn mind Hparam Hfo ind. induction global_adt.
-      [intros; eapply camlValue_to_CoqValue_nil; eauto|].
-      { cbn.  }
-      intros v kn mind Eind Hparam Hfo ind adt Emind Hflag Hind [step Hrel] Hlookup.
-      revert v kn mind Eind Hparam Hfo ind adt Emind Hflag Hind Hrel Hlookup. 
-      induction step; intros; [inversion Hrel|].
-      unfold realize_ADT_gen in Hrel. 
-      apply leb_correct in Hind. simpl in Hrel, Hind. 
-      unfold Nat.ltb in Hrel. rewrite Hind in Hrel.
-      destruct Hrel as [Hrel | Hrel].
-      - apply Existsi_spec in Hrel as [k [Hk [HkS Hrel]]]. cbn in HkS.
-        destruct (filter_firstn _ _ _ _ HkS) as [k' [Hk' Hfilter]].
-        eexists (EAst.tConstruct (mkInd kn ind) k' []); cbn; split.
-        + repeat econstructor. cbn. rewrite Hflag. apply MCProd.andb_and; split; eauto.
-          apply lookup_inductive_env in Hlookup. rewrite Hlookup.
-          pose (MCList.nth_error_spec (EAst.ind_bodies Emind) ind).
-          destruct n.
-          pose (MCList.nth_error_spec (EAst.ind_ctors x) k').
-          destruct n; eauto.  admit. admit. 
-        + rewrite compile_unfold_eq. simpl. 
-          unfold lookup_constructor_args. rewrite Hlookup.
-          subst. unfold EAst.cstr_nargs. admit.
-      - apply Existsi_spec_gen in Hrel as [k [Ts [Hk [HkS [Hrel HTs]]]]]. cbn in HkS.
-        destruct (filter_firstn _ _ _ _ HkS) as [k' [Hk' Hfilter]].
-        destruct Hrel as [v' [eq Hv']].
-
-  
-      pose (map ).
-      eexists (EAst.tConstruct (mkInd kn ind) k' v'); cbn; split.
-      + repeat econstructor. cbn. rewrite Hflag. apply MCProd.andb_and; split; eauto.
-        apply lookup_inductive_env in Hlookup. rewrite Hlookup.
-        pose (MCList.nth_error_spec (EAst.ind_bodies Emind) ind).
-        destruct n.
-        pose (MCList.nth_error_spec (EAst.ind_ctors x) k').
-        destruct n; eauto.  admit. admit. 
-      + rewrite compile_unfold_eq. simpl. 
-        unfold lookup_constructor_args. rewrite Hlookup.
-        subst. unfold EAst.cstr_nargs. admit.
-    
-    
-  
-    destruct 
-    destruct mind.   ind_bodies0; [inversion Hind|].
-    simpl in Hrel. unfold Nat.ltb in Hrel. rewrite Hind in Hrel.
-    - set (filter _ _) in Hrel. remember l.
-      apply Existsi_spec in Hrel as [k [Hk [Hk' Hrel]]]. cbn in Hk'.   
-      eexists (EAst.tConstruct (mkInd kn ind) k []); cbn; split.
-      + repeat econstructor. cbn. admit.
-      + subst. rewrite compile_unfold_eq. simpl. 
-        unfold lookup_constructor_args. rewrite Hlookup. econstructor.
-      + admit.
-    -      
-          apply eval_num_int. econstructor.    
-          unfold EGlobalEnv.lookup_env in Hlookup. 
-
-    2: { unfold firstorder_oneind in Hfo. apply MCProd.andb_and in Hfo. } 
-      unfold CoqType_to_camlType in adt. 
-
-End firstorder.
-
+  intros ? ? ? wfΣ ? ? Hlookup. intros. cbn. rewrite ReflectEq.eqb_refl. cbn.
+  intros t Ht. unfold to_realize_term in *. intros h h' v Heval.
+  assert (Hindmax : (Z.of_nat ind < Int63.wB)%Z).
+  { epose proof (ind_wB mind _ _ _ _); eauto.
+    cbn in H2. rewrite CoqType_to_camlType'_length in H2. lia. }
+  rewrite int_to_of_nat in Ht; eauto. rewrite int_to_of_nat; eauto.
+  pose proof (Hlookup' := Hlookup).
+  unfold lookup_inductive, lookup_inductive_gen, lookup_minductive_gen in Hlookup. cbn in Hlookup.
+  rewrite ReflectEq.eqb_refl in Hlookup.
+  assert (HEind : nth_error (ind_bodies mind) ind = Some Eind).
+  { destruct (nth_error (ind_bodies mind) ind); now inversion Hlookup. }          
+  inversion Heval; subst.
+  - specialize (Ht _ _ _ H8).
+    unshelve eapply camlValue_to_CoqValue_nil in Ht; eauto; cbn.
+    destruct Ht as [t_coq Ht]. specialize (Ht h2). destruct Ht as [Ht_typ Ht_eval].
+    assert (h2 = h').
+    { eapply isPure_heap in H6; try eapply compile_pure; intros; cbn; eauto. cbn in H6. destruct H6 as [[? ? ] ?]. 
+      eapply isPure_heap; try apply H11; intros; cbn; eauto.
+      unfold Ident.Map.add. destruct (Ident.eqb s x); eauto.
+      eapply isPure_heap in Ht_eval; try eapply compile_pure; intros; cbn; eauto. now destruct Ht_typ. }
+    subst. eapply isPure_heap in H6; try eapply compile_pure; intros; cbn; eauto.
+    destruct H6 as [? ?]; subst.  
+    eapply compile_compose in H8; eauto. 
+    2: { eapply isPure_heap_irr,  Ht_eval; try eapply compile_pure; intros; cbn; eauto. }
+    unshelve eapply CoqValue_to_CamlValue; try exact H8; try rewrite int_to_of_nat; eauto.
+    destruct H3, Ht_typ. sq. 
+    unshelve epose proof (type_App _ _ _ _ _ _ _ _ _ X X0); try exact (ind_sort Eind); eauto.
+    rewrite <- (sort_of_product_idem _).
+    assert ((Σ, univ_decl);;; []
+    |- tInd {| inductive_mind := kn; inductive_ind := ind |}
+         [] : tSort (ind_sort Eind)).
+    {  unshelve epose proof (type_Ind (Σ,univ_decl) [] (mkInd kn ind) [] mind Eind _ _ _).
+    *** econstructor.
+    *** unfold declared_constructor, declared_inductive. subst. now cbn.
+    *** unfold consistent_instance_ext, consistent_instance; cbn.
+       now rewrite Hmono.
+    *** unfold ind_type in X1. destruct Eind; cbn in *.
+        unfold PCUICTyping.wf in wfΣ. inversion wfΣ as [_ wfΣ'].
+        cbn in wfΣ'. inversion wfΣ'. clear X2. inversion X3. inversion on_global_decl_d.
+        eapply Alli_nth_error in onInductives; eauto. cbn in onInductives.
+        inversion onInductives. cbn in *.
+        eapply nth_error_forall in Hindices; eauto. cbn in Hindices. rewrite Hindices in ind_arity_eq.                       
+        cbn in ind_arity_eq. rewrite Hparam in ind_arity_eq. cbn in ind_arity_eq.
+        rewrite ind_arity_eq in X1. cbn in X1. admit. }            
+    eapply type_Prod; eauto.
+    unshelve epose proof (type_Ind (Σ,univ_decl) 
+          ([],,vass na (tInd {| inductive_mind := kn; inductive_ind := ind |} [])) (mkInd kn ind) [] mind Eind _ _ _).
+        *** econstructor. econstructor. cbn. unfold infer_sort.
+            eexists; eauto.   
+        *** unfold declared_constructor, declared_inductive. subst. now cbn.
+        *** unfold consistent_instance_ext, consistent_instance; cbn.
+           now rewrite Hmono.
+        *** unfold ind_type in X1. destruct Eind; cbn in *.
+            unfold PCUICTyping.wf in wfΣ. inversion wfΣ as [_ wfΣ'].
+            cbn in wfΣ'. inversion wfΣ'. clear X3. inversion X4. inversion on_global_decl_d.
+            eapply Alli_nth_error in onInductives; eauto. cbn in onInductives.
+            inversion onInductives. cbn in *.
+            eapply nth_error_forall in Hindices; eauto. cbn in Hindices. rewrite Hindices in ind_arity_eq.                       
+            cbn in ind_arity_eq. rewrite Hparam in ind_arity_eq. cbn in ind_arity_eq.
+            rewrite ind_arity_eq in X2. cbn in X2. admit. 
+  - specialize (Ht _ _ _ H7).
+    eapply camlValue_to_CoqValue_nil in Ht; eauto; cbn.
+    destruct Ht as [t_coq Ht].
+    specialize (Ht h2).  destruct Ht as [Ht_typ Ht_eval].
+    assert (h2 = h').
+    { eapply isPure_heap in H6; try eapply compile_pure; intros; cbn; eauto.
+      cbn in H6. destruct H6 as [[? ? ] ?].
+      pose proof (proj1 (Forall_nth _ _) H5 n Bad_recursive_value).
+      rewrite H9 in H8. cbn in H8.
+      eapply isPure_heap in Ht_eval; try eapply compile_pure; intros; cbn; eauto. 
+      destruct Ht_eval as [? _].
+      case_eq (Nat.ltb n #|mfix|); try rewrite Nat.ltb_lt; eauto.
+      intro; eapply isPure_heap; try apply H12; intros; cbn; eauto.
+      unfold Ident.Map.add. destruct (Ident.eqb s y); eauto.
+      cbn. eapply isPure_add_self; eauto.
+      rewrite Nat.ltb_ge. intro neq. rewrite nth_overflow in H9; eauto. inversion H9. }
+    subst. eapply isPure_heap in H6; try eapply compile_pure; intros; cbn; eauto. 
+    destruct H6 as [? ?]; subst.  
+    eapply compile_compose in H7; eauto. 
+    2: { eapply isPure_heap_irr,  Ht_eval; try eapply compile_pure; intros; cbn; eauto. }
+    unshelve eapply CoqValue_to_CamlValue; try exact H7; try rewrite int_to_of_nat; eauto.
+    destruct H3, Ht_typ. sq.
+    unshelve epose proof (type_App _ _ _ _ _ _ _ _ _ t0 X); try exact (ind_sort Eind); eauto. 
+    rewrite <- (sort_of_product_idem _).
+    assert ((Σ, univ_decl);;; []
+    |- tInd {| inductive_mind := kn; inductive_ind := ind |}
+         [] : tSort (ind_sort Eind)).
+    {  unshelve epose proof (type_Ind (Σ,univ_decl) [] (mkInd kn ind) [] mind Eind _ _ _).
+    *** econstructor.
+    *** unfold declared_constructor, declared_inductive. subst. now cbn.
+    *** unfold consistent_instance_ext, consistent_instance; cbn. now rewrite Hmono.
+    *** unfold ind_type in X0. destruct Eind; cbn in *.
+        unfold PCUICTyping.wf in wfΣ. inversion wfΣ as [_ wfΣ'].
+        cbn in wfΣ'. inversion wfΣ'. clear X1. inversion X2. inversion on_global_decl_d.
+        eapply Alli_nth_error in onInductives; eauto. cbn in onInductives.
+        inversion onInductives. cbn in *.
+        eapply nth_error_forall in Hindices; eauto. cbn in Hindices. rewrite Hindices in ind_arity_eq.                       
+        cbn in ind_arity_eq. rewrite Hparam in ind_arity_eq. cbn in ind_arity_eq.
+        rewrite ind_arity_eq in X0. cbn in X0. unfold subst_instance_univ in X0. destruct ind_sort0; eauto.
+        unfold subst_instance, subst_instance_univ0 in X0. unfold subst_instance_level_expr in X0.
+        admit. }            
+    eapply type_Prod; eauto.
+    unshelve epose proof (type_Ind (Σ,univ_decl) 
+          ([],,vass na (tInd {| inductive_mind := kn; inductive_ind := ind |} [])) (mkInd kn ind) [] mind Eind _ _ _).
+        *** econstructor. econstructor. cbn. unfold infer_sort.
+            eexists; eauto.   
+        *** unfold declared_constructor, declared_inductive. subst. now cbn.
+        *** unfold consistent_instance_ext, consistent_instance; cbn.
+           now rewrite Hmono.
+        *** unfold ind_type in X1. destruct Eind; cbn in *.
+            unfold PCUICTyping.wf in wfΣ. inversion wfΣ as [_ wfΣ'].
+            cbn in wfΣ'. inversion wfΣ'. clear X2. inversion X3. inversion on_global_decl_d.
+            eapply Alli_nth_error in onInductives; eauto. cbn in onInductives.
+            inversion onInductives. cbn in *.
+            eapply nth_error_forall in Hindices; eauto. cbn in Hindices. rewrite Hindices in ind_arity_eq.                       
+            cbn in ind_arity_eq. rewrite Hparam in ind_arity_eq. cbn in ind_arity_eq.
+            rewrite ind_arity_eq in X1. cbn in X1. admit. 
+  - rewrite (compile_function _ _ _ _ _ _ _ _ _ H3 H7) in H10. inversion H10.
+  Abort.
